specs/ecdsap256/Spec.ECC.Curves.fst
@@ -160,7 +160,7 @@ let getLongPower curve = getPower curve * 2
 
 (* order of the curves *)
 inline_for_extraction
-let getOrder (#c: curve) : (a: pos{a < pow2 (getPower c) /\ pow2 (getPower c) < 2 * a /\ FStar.Math.Euclid.is_prime a /\ pow2 (getPower c) % a <> 0}) =
+let getOrder (#c: curve) : (a: pos{a > pow2 64 /\ a < pow2 (getPower c) /\ pow2 (getPower c) < 2 * a /\ FStar.Math.Euclid.is_prime a /\ pow2 (getPower c) % a <> 0}) =
   admit();
   match c with 
   |P256 -> assert_norm (115792089210356248762697446949407573529996955224135760342422259061068512044369 < pow2 (getPower P256));
